ttcan: trigger-timely example

example/ttcan/Network.TTCan.TriggerTimely.fst
@@ -4,9 +4,12 @@
      Tx_Ref_Triggers by [-127,127];
   2. we use arbitrary-sized integer arithmetic for indices and times, which
      reduces some syntactic noise;
-  3. we use a simple tick-based time instead of microseconds
+  3. we use a simple tick-based time instead of microseconds;
+  4. no reset trigger;
+  5. cycle offset is assumed constant (rather than taking a new value every reset)
 *)
 module Network.TTCan.TriggerTimely
+#push-options "--print_bound_var_types --print_full_names"
 
 module S     = Pipit.Sugar.Shallow
 
@@ -15,125 +18,137 @@ module SugarTac  = Pipit.Sugar.Shallow.Tactics
 module Check     = Pipit.Sugar.Check
 module T = Pipit.Tactics
 
-module UInt8 = FStar.UInt8
-// module UInt64 = FStar.UInt64
-
 module Ints = Network.TTCan.Prim.IntUnsafe
 
-// module U64S = Network.TTCan.Prim.U64
-
-type index = nat
+type index = int
 (* Tick-based logical time; one message per tick *)
 type time  = int
 (* Cycle index < 64 *)
-type cycle = UInt8.t
+type cycle = int
 
-(* Simple axiomatisation of read-only arrays. I don't think we can generate C code for this *)
 noeq
-type const_array (a: eqtype) = {
-  get: int -> a;
-  size: index;
+type trigger_array = {
+  size:      nat;
+  enabled:   index -> cycle -> bool;
+  time_mark: index -> time;
 }
-
-type trigger = {
-  (* When the trigger should start running *)
-  time_mark:     time;
-  (* Triggers are only enabled on certain cycles. *)
-  (* Cycle_Mask is based on Repeat_Factor: cycle_mask = (1 << repeat_factor) - 1 *)
-  cycle_mask:    cycle;
-  (* Phase / offset *)
-  cycle_offset:  cycle;
-
-  // Missing:
-  // trigger_type: Tx | Rx | Tx_Ref | Watch | ...
-  // message_id: message_id // for Tx and Rx
-}
-
-
-instance has_stream_uint8: S.has_stream UInt8.t = {
-  ty_id       = [`%UInt8.t];
-  val_default = 0uy;
-}
-
-instance has_stream_trigger: S.has_stream trigger = {
-  ty_id       = [`%trigger];
-  val_default = { time_mark = S.val_default; cycle_mask = S.val_default; cycle_offset = S.val_default; };
-}
-
-
-(* Check if a trigger is enabled on a specific cycle index *)
-let trigger_enabled (trigger: trigger) (cycle_index: cycle): bool =
-  (UInt8.logand cycle_index trigger.cycle_mask) = trigger.cycle_offset
 
 (*** Time-marks are sorted:
   The time-marks in an array must be *nondecreasingly* sorted. Duplicate
   time-marks are allowed, as long the two triggers are not enabled in the same
   cycle (formalised below).
 *)
-let time_mark_sorted_req (triggers: const_array trigger): prop =
+let time_mark_sorted_req (triggers: trigger_array): prop =
   forall (i: index { i < triggers.size - 1 }).
-    (triggers.get i).time_mark <= (triggers.get (i + 1)).time_mark
-
+    triggers.time_mark i <= triggers.time_mark (i + 1)
 
 (*** Adequate spacing:
   If two triggers, i and j, are enabled in the same cycle, then their time
   marks must be far enough apart that we have time to iterate through the
   indices from i to j.
 *)
-let adequate_spacing (triggers: const_array trigger) (i j: index) (c: cycle): prop =
+let adequate_spacing (triggers: trigger_array) (i j: nat) (c: cycle): prop =
   i < triggers.size                  ==>
   j < triggers.size                  ==>
   i <= j                             ==>
-  trigger_enabled (triggers.get i) c ==>
-  trigger_enabled (triggers.get j) c ==>
-  (triggers.get j).time_mark - (triggers.get i).time_mark >= (j - i)
+  triggers.enabled i c               ==>
+  triggers.enabled j c               ==>
+  (triggers.time_mark j - triggers.time_mark i) >= (j - i)
 
-let adequate_spacing_req (triggers: const_array trigger): prop =
-  forall (i j: index). forall (c: cycle).
+let adequate_spacing_req (triggers: trigger_array): prop =
+  forall (i j: nat). forall (c: cycle).
     adequate_spacing triggers i j c
 
 (*** Time-marks are reachable from start:
   After a reset, we need to be able to get from index 0 to the first enabled
   time-mark i before it starts. This should hold in general too.
 *)
-let time_mark_reachable_req (triggers: const_array trigger): prop =
-  forall (i: index { i < triggers.size }).
-    i <= (triggers.get i).time_mark
+let time_mark_reachable_req (triggers: trigger_array): prop =
+  forall (i: index { 0 <= i /\ i < triggers.size }).
+    i <= triggers.time_mark i
 
-(* Static trigger configuration, with proofs of the above properties *)
+(* Static trigger configuration with proofs of the above properties *)
 noeq
 type config = {
-  triggers: tr: const_array trigger { tr.size > 0 };
+  triggers:                trigger_array;
   time_mark_sorted_req:    squash (time_mark_sorted_req triggers);
   adequate_spacing_req:    squash (adequate_spacing_req triggers);
   time_mark_reachable_req: squash (time_mark_reachable_req triggers);
+  size_req:                squash (triggers.size > 0);
 }
 
 
-(* Find next enabled trigger, or triggers.size if none enabled *)
-let rec next (triggers: const_array trigger) (ix: index { ix <= triggers.size }) (c: cycle)
-  : Tot (j: index { ix <= j /\ j <= triggers.size /\ (trigger_enabled (triggers.get j) c \/ j == triggers.size)}) (decreases (triggers.size - ix)) =
-  if trigger_enabled (triggers.get ix) c
-  then ix
-  else if ix < triggers.size - 1
-  then next triggers (ix + 1) c
-  else triggers.size // reached end
+(* Find next enabled trigger or None *)
+let rec next (triggers: trigger_array) (ix: int) (c: cycle)
+  : Tot (option (j: index { j < triggers.size /\ (triggers.enabled j c) /\ ix <= j })) (decreases (triggers.size - ix)) =
+  if ix < 0 || ix >= triggers.size
+  then None
+  else if triggers.enabled ix c
+  then Some ix
+  else (
+    match next triggers (ix + 1) c with
+    | Some i -> Some i
+    | None -> None
+  )
 
-(* No enabled triggers remain *)
-let next_none (cfg: config) (ix: index { ix < cfg.triggers.size }) (c: cycle): prop =
-  next cfg.triggers ix c == cfg.triggers.size
+let trigger_index_invariant (cfg: config) (c: cycle) (now: time) (index: index): bool =
+  match next cfg.triggers index c with
+  | None -> true
+  | Some n -> (cfg.triggers.time_mark n - now) >= (n - index)
 
-let lemma_next_monotonic (triggers: const_array trigger) (ix: index { ix < triggers.size }) (c: cycle)
-  : Lemma (next triggers ix c <= next triggers (ix + 1) c)
+let trigger_index_invariant_base (cfg: config) (c: cycle)
+  : Lemma (trigger_index_invariant cfg c 0 0) =
+  ()
+
+let trigger_index_invariant_stay (cfg: config) (c: cycle) (now: int) (index: int)
+  : Lemma (
+      (trigger_index_invariant cfg c now index /\
+      cfg.triggers.enabled index c /\
+      cfg.triggers.time_mark index > now)
+    ==>
+      (trigger_index_invariant cfg c (now + 1) index)) =
+  ()
+
+let lemma_adequate_spacing_next_inc_def (cfg: config) (c: cycle) (index: index) =
+  match next cfg.triggers (index + 1) c with
+  | None -> True
+  | Some n ->
+    0 <= index ==>
+    adequate_spacing cfg.triggers index n c
+
+let lemma_adequate_spacing_next_inc (cfg: config) (c: cycle)
+  : Lemma (forall (index: index). lemma_adequate_spacing_next_inc_def cfg c index)
   = ()
 
-let trigger_index_invariant (cfg: config) (c: cycle) (now: int) (index: int): prop =
-  0 <= index /\ index <= cfg.triggers.size /\
-  (let n = next cfg.triggers index c in
-    n < cfg.triggers.size ==>
-    (index < cfg.triggers.size /\ (cfg.triggers.get n).time_mark - now >= (n - index)))
+let trigger_index_invariant_step (cfg: config) (c: cycle) (now: int) (index: int)
+  : Lemma (
+      (0 <= index /\ trigger_index_invariant cfg c now index)
+    ==>
+      trigger_index_invariant cfg c (now + 1) (index + 1)) =
+  match next cfg.triggers (index + 1) c with
+  | None -> ()
+  | Some n' -> lemma_adequate_spacing_next_inc cfg c
 
-let count_when_unchecked (max: index) (inc: S.stream bool): S.stream int =
+let pose_trigger_index_invariant_zero (cfg: config) (c: cycle): S.stream unit =
+  S.pose (trigger_index_invariant cfg c 0 0)
+    ()
+
+let pose_trigger_index_invariant_stay (cfg: config) (c: cycle) (now: S.stream int) (index: S.stream int): S.stream unit =
+  S.pose2 (fun now index ->
+      (trigger_index_invariant cfg c now index /\
+      cfg.triggers.enabled index c /\
+      cfg.triggers.time_mark index > now)
+    ==>
+      (trigger_index_invariant cfg c (now + 1) index))
+    (fun now index -> trigger_index_invariant_stay cfg c now index)
+    now index
+
+let pose_trigger_index_invariant_step (cfg: config) (c: cycle) (now: S.stream int) (index: S.stream int): S.stream unit =
+  S.pose2
+    (fun now index -> (0 <= index /\ trigger_index_invariant cfg c now index) ==> trigger_index_invariant cfg c (now + 1) (index + 1))
+    (fun now index -> trigger_index_invariant_step cfg c now index) now index
+
+let count_when_unchecked (max: nat) (inc: S.stream bool): S.stream int =
   let open S in
   let open Ints in
   rec' (fun count ->
@@ -141,7 +156,7 @@ let count_when_unchecked (max: index) (inc: S.stream bool): S.stream int =
     let^ count' = (0 `fby` count) + (if_then_else inc (const 1) (const 0)) in
     if_then_else (count' > const max) (const max) count')
 
-let count_when (max: index): S.stream bool -> S.stream int =
+let count_when (max: nat): S.stream bool -> S.stream int =
   let e = Check.exp_of_stream1 (count_when_unchecked max) in
   assert (Check.system_induct_k1 e) by (T.norm_full ["Network"]);
   Check.stream_of_checked1 e
@@ -153,71 +168,64 @@ let time_increasing (now: S.stream int): S.stream bool =
   now = 0 `fby` (now + const 1)
 
 
-let trigger_enabled' (tr: S.stream trigger) (c: cycle): S.stream bool =
-  S.lift1 (fun t -> trigger_enabled t c) tr
+let trigger_enabled (cfg: config) (index: S.stream index) (c: cycle): S.stream bool =
+  S.lift1 (fun index -> cfg.triggers.enabled index c) index
 
-let get_time_mark (tr: S.stream trigger): S.stream time =
-  S.lift1 (fun t -> t.time_mark) tr
+let trigger_time_mark (cfg: config) (index: S.stream index): S.stream time =
+  S.lift1 (fun index -> cfg.triggers.time_mark index) index
 
-let trigger_index (cfg: config) (index: S.stream int): S.stream trigger =
-  S.lift1 cfg.triggers.get index
 
-let trigger_fetch_ctr (c: cycle) =
+let trigger_fetch_unchecked (cfg: config) (c: cycle) (now: S.stream time): S.stream (index & bool) #_ =
   let open S in
   let open Ints in
-  Check.contract Pipit.Prim.Shallow.table [shallow int] (shallow trigger)
-    (Check.exp_of_stream1 time_increasing)
-    (Check.exp_of_stream2 (fun tr now -> trigger_enabled' tr c ==> get_time_mark tr >= now))
-
-let assume_time_increasing: S.stream int -> S.stream unit =
-  let e = Check.exp_of_stream1 (fun now -> S.check "" (time_increasing now)) in
-  assume (Check.system_induct_k1 e);
-  Check.stream_of_checked1 e
-
-let trigger_fetch_unchecked (cfg: config) (c: cycle) (now: S.stream int): S.stream (trigger & int) =
-  let open S in
-  let open Ints in
-  assume_time_increasing now;^
-  rec' (fun trigger_ret ->
-    let trigger = fst trigger_ret in
-    let^ inc = false `fby` ((get_time_mark trigger <= now \/ ~ (trigger_enabled' trigger c))) in
+  rec' (fun index_intr ->
+    let^ index = fst index_intr in
+    let^ inc = false `fby` ((trigger_time_mark cfg index <= now \/ ~ (trigger_enabled cfg index c))) in
     let^ index = count_when cfg.triggers.size inc in
-    let^ trigger = trigger_index cfg index in
+    let^ interrupt = inc /\ index < const cfg.triggers.size /\ trigger_enabled cfg index c in
 
-    check2 (fun now index -> trigger_index_invariant cfg c now index) now index;^
-    tup trigger index)
+    pose1_forall (fun i -> lemma_adequate_spacing_next_inc_def cfg c i) () index;^
+    check "" (sofar (time_increasing now) ==> (lift2 (fun now index -> trigger_index_invariant cfg c now index)) now index);^
+    // pose_trigger_index_invariant_zero cfg c;^
+    // pose_trigger_index_invariant_stay cfg c now index;^
+    // pose_trigger_index_invariant_step cfg c now index;^
+    tup index interrupt)
 
-let trigger_fetch (cfg: config) (c: cycle): S.stream int -> S.stream (trigger & int) =
-  // unpacking cfg and triggers reduces a lot of matches in the generated goals; maybe simplify_products tactic chould break apart records too
-  // match cfg with
-  // | { triggers; time_mark_sorted_req; adequate_spacing_req; time_mark_reachable_req; } ->
-  // match triggers with
-  // | { get; size } ->
-  //   let e = Check.exp_of_stream1 (trigger_fetch_unchecked { triggers = { get; size; }; time_mark_sorted_req; adequate_spacing_req; time_mark_reachable_req; } c) in
-    let e = Check.exp_of_stream1 (trigger_fetch_unchecked cfg c) in
-    let sys = Pipit.System.Exp.system_of_exp e in
-    assert (Pipit.System.Ind.base_case sys) by (T.pipit_simplify_products ["Network.TTCan"]);
-    assert (Pipit.System.Ind.step_case sys) by (T.pipit_simplify_products ["Network.TTCan"]);
-    assert (Check.system_induct_k1 e);
-    Check.stream_of_checked1 e
 
-let trigger_fetch_spec_unchecked (cfg: config) (c: cycle) (now: S.stream int): S.stream (trigger & int) =
-  let trigger_max_index: index = cfg.triggers.size - 1 in
-  let open S in
-  let open Ints in
-  let^ trigger_ret = trigger_fetch cfg c now in
-  let^ trigger = fst trigger_ret in
-  let^ index = snd trigger_ret in
-  let^ new_trigger = index <> (-1) `fby` index in
-  check "" (
-    (new_trigger /\ trigger_enabled' trigger c /\ index < const cfg.triggers.size) ==>
-    get_time_mark trigger >= now);^
-  trigger_ret
-
-let trigger_fetch_spec (cfg: config) (c: cycle): S.stream int -> S.stream (trigger & int) =
+let trigger_fetch (cfg: config) (c: cycle): S.stream time -> S.stream (index & bool) #_ =
   let e = Check.exp_of_stream1 (trigger_fetch_unchecked cfg c) in
   let sys = Pipit.System.Exp.system_of_exp e in
-  assert (Pipit.System.Ind.base_case sys) by (T.pipit_simplify_products ["Network.TTCan"]);
-  assert (Pipit.System.Ind.step_case sys) by (T.pipit_simplify_products ["Network.TTCan"]);
-  assert (Check.system_induct_k1 e);
+  // assert (Pipit.System.Ind.base_case sys) by (T.clear_all (); T.pipit_simplify_products ["Network.TTCan"]; T.dump "base");
+  // assert (Pipit.System.Ind.step_case sys) by (T.clear_all (); T.pipit_simplify_products ["Network.TTCan"]; T.dump "step");
+  assert (Check.system_induct_k1 e) by (T.clear_all (); T.pipit_simplify_products ["Network.TTCan"]; T.dump "check");
   Check.stream_of_checked1 e
+
+
+// let trigger_fetch_ctr (c: cycle) =
+//   let open S in
+//   let open Ints in
+//   Check.contract Pipit.Prim.Shallow.table [shallow time] (shallow index)
+//     (Check.exp_of_stream1 time_increasing)
+//     (Check.exp_of_stream2 (fun index now -> trigger_enabled index c ==> trigger_time_mark index >= now))
+
+
+// let trigger_fetch_spec_unchecked (cfg: config) (c: cycle) (now: S.stream int): S.stream (trigger & int) =
+//   let trigger_max_index: index = cfg.triggers.size - 1 in
+//   let open S in
+//   let open Ints in
+//   let^ trigger_ret = trigger_fetch cfg c now in
+//   let^ trigger = fst trigger_ret in
+//   let^ index = snd trigger_ret in
+//   let^ new_trigger = index <> (-1) `fby` index in
+//   check "" (
+//     (new_trigger /\ trigger_enabled' trigger c /\ index < const cfg.triggers.size) ==>
+//     get_time_mark trigger >= now);^
+//   trigger_ret
+
+// let trigger_fetch_spec (cfg: config) (c: cycle): S.stream int -> S.stream (trigger & int) =
+//   let e = Check.exp_of_stream1 (trigger_fetch_unchecked cfg c) in
+//   let sys = Pipit.System.Exp.system_of_exp e in
+//   assert (Pipit.System.Ind.base_case sys) by (T.pipit_simplify_products ["Network.TTCan"]);
+//   assert (Pipit.System.Ind.step_case sys) by (T.pipit_simplify_products ["Network.TTCan"]);
+//   assert (Check.system_induct_k1 e);
+//   Check.stream_of_checked1 e
